repatch/repatch3_generated.c
@@ -33,7 +33,7 @@ static int get_immediate(unsigned long long ins)
 
 static unsigned long long eval_immediate(int ins)
 {
-  return (unsigned long long) (unsigned int) ins;
+  return (unsigned long long) ins;
 }
 
 static unsigned char get_opcode_ins(unsigned long long ins)
@@ -302,38 +302,31 @@ static void step_opcode_alu32(struct bpf_state* st, unsigned int dst32, unsigned
   opcode_alu32 = get_opcode_alu32(op);
   switch (opcode_alu32) {
     case 0:
-      upd_reg(st, dst,
-              (unsigned long long) (unsigned int) (dst32 + src32));
+      upd_reg(st, dst, (unsigned long long) (dst32 + src32));
       return;
     case 16:
-      upd_reg(st, dst,
-              (unsigned long long) (unsigned int) (dst32 - src32));
+      upd_reg(st, dst, (unsigned long long) (dst32 - src32));
       return;
     case 32:
-      upd_reg(st, dst,
-              (unsigned long long) (unsigned int) (dst32 * src32));
+      upd_reg(st, dst, (unsigned long long) (dst32 * src32));
       return;
     case 48:
       if (src32 != 0U) {
-        upd_reg(st, dst,
-                (unsigned long long) (unsigned int) (dst32 / src32));
+        upd_reg(st, dst, (unsigned long long) (dst32 / src32));
         return;
       } else {
         upd_flag(st, -9);
         return;
       }
     case 64:
-      upd_reg(st, dst,
-              (unsigned long long) (unsigned int) (dst32 | src32));
+      upd_reg(st, dst, (unsigned long long) (dst32 | src32));
       return;
     case 80:
-      upd_reg(st, dst,
-              (unsigned long long) (unsigned int) (dst32 & src32));
+      upd_reg(st, dst, (unsigned long long) (dst32 & src32));
       return;
     case 96:
       if (src32 < 32U) {
-        upd_reg(st, dst,
-                (unsigned long long) (unsigned int) (dst32 << src32));
+        upd_reg(st, dst, (unsigned long long) (dst32 << src32));
         return;
       } else {
         upd_flag(st, -10);
@@ -341,8 +334,7 @@ static void step_opcode_alu32(struct bpf_state* st, unsigned int dst32, unsigned
       }
     case 112:
       if (src32 < 32U) {
-        upd_reg(st, dst,
-                (unsigned long long) (unsigned int) (dst32 >> src32));
+        upd_reg(st, dst, (unsigned long long) (dst32 >> src32));
         return;
       } else {
         upd_flag(st, -10);
@@ -350,7 +342,7 @@ static void step_opcode_alu32(struct bpf_state* st, unsigned int dst32, unsigned
       }
     case 128:
       if (op == 132) {
-        upd_reg(st, dst, (unsigned long long) (unsigned int) -dst32);
+        upd_reg(st, dst, (unsigned long long) -dst32);
         return;
       } else {
         upd_flag(st, -1);
@@ -358,25 +350,21 @@ static void step_opcode_alu32(struct bpf_state* st, unsigned int dst32, unsigned
       }
     case 144:
       if (src32 != 0U) {
-        upd_reg(st, dst,
-                (unsigned long long) (unsigned int) (dst32 % src32));
+        upd_reg(st, dst, (unsigned long long) (dst32 % src32));
         return;
       } else {
         upd_flag(st, -9);
         return;
       }
     case 160:
-      upd_reg(st, dst,
-              (unsigned long long) (unsigned int) (dst32 ^ src32));
+      upd_reg(st, dst, (unsigned long long) (dst32 ^ src32));
       return;
     case 176:
-      upd_reg(st, dst, (unsigned long long) (unsigned int) src32);
+      upd_reg(st, dst, (unsigned long long) src32);
       return;
     case 192:
       if (src32 < 32U) {
-        upd_reg(st, dst,
-                (unsigned long long) (unsigned int) ((int) dst32
-                                                      >> src32));
+        upd_reg(st, dst, (unsigned long long) ((int) dst32 >> src32));
         return;
       } else {
         upd_flag(st, -10);
