model/CommonLib.v
@@ -1,0 +1,186 @@
+From compcert Require Import Coqlib Integers AST Values Memory Ctypes Archi.
+From Coq Require Import Lia ZArith.
+
+Open Scope Z_scope.
+
+
+Lemma Int64_max_unsigned_eq:
+  Int64.max_unsigned = 18446744073709551615.
+Proof.
+  unfold Int64.max_unsigned, Int64.modulus, Int64.wordsize, Wordsize_64.wordsize; reflexivity.
+Qed.
+
+Lemma Int_max_unsigned_eq:
+  Int.max_unsigned = 4294967295.
+Proof.
+  unfold Int.max_unsigned, Int.modulus, Int.wordsize, Wordsize_32.wordsize; reflexivity.
+Qed.
+
+Lemma size_chunk_gt_zero:
+  forall chunk, 0 < size_chunk chunk.
+Proof.
+  intros.
+  unfold size_chunk.
+  destruct chunk; try lia.
+Qed.
+
+Lemma size_chunk_int_range:
+  forall chunk, 0 <= size_chunk chunk <= Int.max_unsigned.
+Proof.
+  unfold size_chunk; intros.
+  rewrite Int_max_unsigned_eq.
+  split; destruct chunk; try lia.
+Qed.
+
+(*
+Lemma _32_lt_64:
+  Int.ltu int32_32 Int64.iwordsize' = true.
+Proof.
+  unfold int32_32, Int64.iwordsize'.
+  unfold Int64.zwordsize, Int64.wordsize, Wordsize_64.wordsize.
+  unfold Int.ltu.
+  simpl.
+  assert (H0: 0 <= 32 <= Int.max_unsigned).
+  unfold Int.max_unsigned, Int.modulus, Int.wordsize, Wordsize_32.wordsize; simpl; lia.
+  assert (H1: 0 <= 64 <= Int.max_unsigned).
+  unfold Int.max_unsigned, Int.modulus, Int.wordsize, Wordsize_32.wordsize; simpl; lia.
+  rewrite Int.unsigned_repr; try assumption.
+  rewrite Int.unsigned_repr; try assumption.
+  simpl; reflexivity.
+Qed.
+
+Lemma sint16_to_int64_to_vlong:
+  forall ofs,
+    exists v, int64_to_vlong (sint16_to_int64 ofs) = Vlong v.
+Proof.
+  unfold int64_to_vlong, sint16_to_int64; intros.
+  exists (Int64.repr (Int16.Int16.signed ofs)); reflexivity.
+Qed. *)
+
+Lemma Int64_unsigned_ge_0:
+  forall v, 0 <= Int64.unsigned v.
+Proof.
+  intro v.
+  assert (Hrange: 0 <= Int64.unsigned v <= Int64.max_unsigned). {
+    apply Int64.unsigned_range_2.
+  }
+  destruct Hrange as [Ha Hb]; assumption.
+Qed.
+
+Lemma Int_repr_zero:
+  forall v, 0<=v<=Int.max_unsigned -> Int.unsigned (Int.repr v) = Int.unsigned (Int.zero) -> v = 0.
+Proof.
+  intros.
+  rewrite (Int.unsigned_repr v H) in H0.
+  rewrite Int.unsigned_zero in H0.
+  assumption.
+Qed.
+
+Lemma Ptrofs_of_int_unsigned:
+  forall v, Ptrofs.unsigned (Ptrofs.of_int v) = Int.unsigned v.
+Proof.
+  intros.
+  assert (H1: Ptrofs.agree32 (Ptrofs.of_int v) v). { apply Ptrofs.agree32_of_int. reflexivity. }
+  rewrite H1; reflexivity.
+Qed.
+
+Lemma ptrofs_unsigned_ge_0:
+  forall v, 0 <= Ptrofs.unsigned v.
+Proof.
+  intro v.
+  assert (Hrange: 0 <= Ptrofs.unsigned v <= Ptrofs.max_unsigned). {
+    apply Ptrofs.unsigned_range_2.
+  }
+  destruct Hrange as [Ha Hb]; assumption.
+Qed.
+
+Lemma Cle_implies_Zle:
+  forall lo ofs,
+    negb (Int64.ltu ofs lo) = true ->
+      Int64.unsigned lo <= Int64.unsigned ofs.
+Proof.
+  intros.
+  rewrite negb_true_iff in H.
+  unfold Int64.ltu in H.
+  destruct (zlt _ _) in H; try inversion H.
+  lia.
+Qed.
+
+Lemma Clt_implies_Zlt:
+  forall ofs hi,
+    Int64.ltu ofs hi = true ->
+      Int64.unsigned ofs < Int64.unsigned hi.
+Proof.
+  intros.
+  unfold Int64.ltu in H.
+  destruct (zlt _ _) in H; try inversion H.
+  lia.
+Qed.
+
+Lemma unsigned_size_chunk_ge_0:
+  forall ofs chunk,
+    0 <= Int64.unsigned ofs + size_chunk chunk.
+Proof.
+  intros.
+  assert (Hchunk_lo: 0 < size_chunk chunk). apply size_chunk_gt_zero.
+  assert (Hofs_lo: 0<= Int64.unsigned ofs). apply Int64_unsigned_ge_0. 
+  unfold size_chunk; destruct chunk; rewrite Z.add_comm; try lia.
+Qed.
+
+Lemma unsigned_ofs_size_chunk_ge_0:
+  forall ofs chunk,
+    Int64.unsigned ofs < Int64.unsigned ofs + size_chunk chunk.
+Proof.
+  intros.
+  assert (Hchunk_lo: 0 < size_chunk chunk). apply size_chunk_gt_zero.
+  assert (Hofs_lo: 0<= Int64.unsigned ofs). apply Int64_unsigned_ge_0. 
+  lia.
+Qed.
+
+(**r Here is a problem, 'ofs+size_chunk':Z may be greater than Int64.mex_unsigned! 
+     While the 'Vlong (Int64.repr (ofs+size_chunk))': Val is always within the range!
+ *)
+(*
+Lemma hi_ofs_max_unsigned:
+  forall ofs chunk,
+    negb
+         (Int64.ltu (Int64.repr (Int64.max_unsigned-(size_chunk chunk))) ofs) = true ->
+      0 <= Int64.unsigned ofs + size_chunk chunk <= Int64.max_unsigned.
+Proof.
+  intros ofs chunk Hcmp.
+  rewrite Int64_max_unsigned_eq in *.
+  remember ((Int64.ltu (Int64.repr (18446744073709551615 - size_chunk chunk))) ofs) as k eqn: Hk.
+  rewrite Hk in Hcmp; clear Hk.
+  rewrite negb_true_iff in Hcmp.
+  unfold Int64.ltu in Hcmp.
+  destruct (zlt _ _) in Hcmp.
+  - inversion Hcmp.
+  - clear Hcmp.
+    assert (Heq_max: 0 <= 18446744073709551615 - size_chunk chunk <= Int64.max_unsigned). {
+      rewrite Int64_max_unsigned_eq.
+      unfold size_chunk; destruct chunk; try lia.
+    }
+    rewrite (Int64.unsigned_repr _ Heq_max) in g.
+    split.
+    apply unsigned_size_chunk_ge_0.
+    lia.
+Qed.
+
+Lemma Clt_implies_Zlt_add:
+  forall ofs chunk hi, Int64.ltu (Int64.add ofs (Int64.repr (size_chunk chunk))) hi = true ->
+    0 <= (Int64.unsigned ofs + size_chunk chunk) <= Int64.max_unsigned ->
+      0<= Int64.unsigned ofs + (size_chunk chunk) < Int64.unsigned hi.
+Proof.
+  intros.
+  split.
+  apply unsigned_size_chunk_ge_0.
+  unfold Int64.ltu, Int64.add in H.
+  destruct (zlt _ _) in H; try inversion H.
+  assert (H5: Int64.unsigned (Int64.repr (size_chunk chunk)) = size_chunk chunk). { apply Int64.unsigned_repr; apply size_chunk_int64_range; assumption. }
+  rewrite H5 in l.
+  assert (H6: Int64.unsigned (Int64.repr (Int64.unsigned ofs + size_chunk chunk)) = 
+              (Int64.unsigned ofs + size_chunk chunk)). { apply Int64.unsigned_repr; assumption. }
+  rewrite H6 in l; assumption.
+Qed.
+*)
+Close Scope Z_scope.
