model/Isolation.v
@@ -1,0 +1,29 @@
+From compcert Require Import Values.
+From bpf.comm Require Import State Monad.
+From bpf.model Require Import Syntax Semantics CommonLib AlignChunk RegsInv MemInv.
+
+Theorem step_preserving_inv:
+  forall st1 st2
+    (Hreg: register_inv st1)
+    (Hmem: memory_inv st1)
+    (Hsem: step st1 = Some (tt, st2)),
+       register_inv st2 /\ memory_inv st2.
+Proof.
+  unfold step.
+Ltac unfold_monad :=
+  match goal with
+  | |- _ =>
+    unfold bindM, eval_pc, eval_ins, decodeM, upd_reg, upd_pc, upd_pc_incr, eval_reg, eval_ins_len, get_immediate, returnM
+  end.
+  unfold_monad.
+  intros.
+  destruct (Decode.decode _) in Hsem.
+  - (* BPF_NEG *)
+    apply reg_inv_eval_reg with (r:= r) in Hreg as Heval_reg.
+    destruct Heval_reg as (vl & Heval_reg).
+    destruct a; rewrite Heval_reg in Hsem; simpl in Hsem.
+    + split.
+      inversion Hsem.
+      eapply reg_inv_upd_reg; eauto.
+      TBC.
+Qed.
