model/RegsInv.v
@@ -1,0 +1,168 @@
+From bpf.comm Require Import Regs State.
+From compcert Require Import Values.
+
+Definition is_vlong (v: val): Prop :=
+  match v with
+  | Vlong _ => True
+  | _ => False
+  end.
+
+Definition register_inv (st: state): Prop :=
+  is_vlong (r0_val  (regs_st st)) /\
+  is_vlong (r1_val  (regs_st st)) /\
+  is_vlong (r2_val  (regs_st st)) /\
+  is_vlong (r3_val  (regs_st st)) /\
+  is_vlong (r4_val  (regs_st st)) /\
+  is_vlong (r5_val  (regs_st st)) /\
+  is_vlong (r6_val  (regs_st st)) /\
+  is_vlong (r7_val  (regs_st st)) /\
+  is_vlong (r8_val  (regs_st st)) /\
+  is_vlong (r9_val  (regs_st st)) /\
+  is_vlong (r10_val (regs_st st)).
+
+Lemma is_vlong_iff:
+  forall v,
+    is_vlong v <->
+      exists vl,
+        v = Vlong vl.
+Proof.
+  unfold is_vlong; split; intros.
+  - destruct v; try intuition.
+    exists i; reflexivity.
+  - destruct H as (vl & H).
+    rewrite H.
+    constructor.
+Qed.
+
+Lemma reg_inv_init: register_inv init_state.
+Proof.
+  unfold register_inv, init_state.
+  repeat split.
+Qed.
+
+Lemma reg_inv_eval_reg:
+  forall st r
+    (Hreg_inv: register_inv st),
+    exists i,
+      eval_reg r st = Vlong i.
+Proof.
+  intros.
+  unfold register_inv in Hreg_inv.
+  apply is_vlong_iff.
+  unfold eval_reg.
+  unfold eval_regmap.
+  destruct r; intuition.
+Qed.
+
+Lemma reg_inv_upd_reg:
+  forall st1 st2 r n
+    (Hreg_inv: register_inv st1)
+    (Halu: upd_reg r (Vlong n) st1 = st2),
+      register_inv st2.
+Proof.
+  unfold register_inv, upd_reg, upd_regmap.
+  intros.
+  rewrite <- Halu.
+  destruct r; simpl; tauto.
+Qed.
+
+Lemma reg_inv_upd_flag:
+  forall st1 st2 f
+    (Hreg_inv: register_inv st1)
+    (Hflag: upd_flag f st1 = st2),
+      register_inv st2.
+Proof.
+  unfold register_inv, upd_flag, upd_regmap.
+  intros.
+  rewrite <- Hflag.
+  simpl.
+  assumption.
+Qed.
+
+Lemma reg_inv_upd_mem:
+  forall st1 st2 m
+    (Hreg_inv: register_inv st1)
+    (Hmem: upd_mem m st1 = st2),
+      register_inv st2.
+Proof.
+  unfold register_inv.
+  intros.
+  rewrite <- Hmem.
+  unfold upd_mem.
+  simpl; assumption.
+Qed.
+
+Lemma reg_inv_upd_pc:
+  forall st1 st2 p
+    (Hreg_inv: register_inv st1)
+    (Hpc: upd_pc p st1 = st2),
+      register_inv st2.
+Proof.
+  unfold register_inv.
+  intros.
+  rewrite <- Hpc.
+  unfold upd_pc.
+  simpl; assumption.
+Qed.
+
+Lemma reg_inv_upd_pc_incr:
+  forall st1 st2
+    (Hreg_inv: register_inv st1)
+    (Hpc: upd_pc_incr st1 = st2),
+      register_inv st2.
+Proof.
+  unfold register_inv.
+  intros.
+  rewrite <- Hpc.
+  unfold upd_pc.
+  simpl; assumption.
+Qed.
+
+Lemma reg_inv_eval_src:
+  forall st r,
+    register_inv st ->
+      exists vl,
+        eval_reg r st = Vlong vl.
+Proof.
+  unfold register_inv, eval_reg, eval_regmap.
+  intros.
+  rewrite <- is_vlong_iff.
+  destruct r; intuition.
+Qed.
+(*
+Lemma reg_inv_upd_reg_eval_flag:
+  forall st1 st2 r v
+    (Hreg: upd_reg r v st1 = st2),
+      eval_flag st1 = eval_flag st2.
+Proof.
+  intros.
+  rewrite <- Hreg.
+  unfold upd_reg, eval_flag.
+  simpl.
+  reflexivity.
+Qed.
+
+Lemma reg_inv_upd_pc_eval_flag:
+  forall st1 st2 p
+    (Hpc: upd_pc p st1 = st2),
+      eval_flag st1 = eval_flag st2.
+Proof.
+  intros.
+  rewrite <- Hpc.
+  unfold upd_pc, eval_flag.
+  simpl.
+  reflexivity.
+Qed.
+
+Lemma reg_inv_upd_pc_incr_eval_flag:
+  forall st1 st2
+    (Hpc: upd_pc_incr st1 = st2),
+      eval_flag st1 = eval_flag st2.
+Proof.
+  intros.
+  rewrite <- Hpc.
+  unfold upd_pc_incr, eval_flag.
+  simpl.
+  reflexivity.
+Qed.
+*)
